typing for rules; reworked substitutions

ModularEngine/src/LogicEngine.FStar/interp.fst
@@ -5,28 +5,57 @@ open Marshall
 open State
 open Subst
 
-type vars = list var
-type substitutions = list substitution
-
 let me = Crypto.lookup_my_credentials () 
+
+type infon = polyterm
+type communication = i:infon{Net.Received i}
+type communications = list communication
 
 type condition =
   | If   : polyterm -> condition
   | Upon : polyterm -> condition
-
 type conditions = list condition
+type WFCond :: vars => condition => P =
+  | WFCond_If: xs:vars -> i:infon 
+            -> Typing.polytyping xs i 
+            -> WFCond xs (If i)
+  | WFCond_Upon: xs:vars -> i:infon 
+            -> Typing.polytyping xs i 
+            -> WFCond xs (Upon i)
+logic function Vars : polyterm -> vars 
+assume forall (xs:vars) (i:term). (Vars (ForallT xs i))=(FreeVars i)
+assume forall (xs:vars) (i:term). (Vars (MonoTerm i))=(FreeVars i)
+logic function VarsCond : condition -> vars
+assume forall (i:polyterm). (VarsCond (If i)) = (Vars i)
+assume forall (i:polyterm). (VarsCond (Upon i)) = (Vars i)
+logic function VarsConds : conditions -> vars
+assume Vars_nil: (VarsConds [])=[]
+assume Vars_cons: forall (c:condition) (cs:conditions). (VarsConds (c::cs))=(Append (VarsCond c) (VarsConds cs))
+type Binds :: conditions => vars => E
+assume (forall (cs:conditions) (xs:vars). Includes (VarsConds cs) xs => Binds cs xs)
 
 type action =
   | Learn : polyterm -> action (* infon *)
   | Drop  : polyterm -> action (* infon *)
   | Fwd   : term -> polyterm -> action (* prin, infon *)
   | Send  : term -> polyterm -> action (* prin, infon *)
-
 type actions = list action
+type WFAct :: vars => action => P =
+  | WFAct_Learn: xs:vars -> i:infon 
+              -> Typing.polytyping xs i 
+              -> WFAct xs (Learn i)
+  | WFAct_Drop : xs:vars -> i:infon 
+              -> Typing.polytyping xs i 
+              -> WFAct xs (Drop i)
+  | WFAct_Fwd  : xs:vars -> p:term -> i:infon 
+              -> Typing.typing xs p Principal
+              -> Typing.polytyping xs i 
+              -> WFAct xs (Fwd p i)
+  | WFAct_Send : xs:vars -> p:term -> i:infon 
+              -> Typing.typing xs p Principal
+              -> Typing.polytyping xs i 
+              -> WFAct xs (Send p i)
 
-type infon = polyterm
-type communication = i:infon{Net.Received i}
-type communications = list communication
 
 (* -------------------------------------------------------------------------------- *)
 (* Spec: Validity of condition(s) *)
@@ -45,25 +74,22 @@ type HoldsOne :: substitution => vars => condition => substitution => E
 assume Holds_if: forall (xs:vars) (i:infon) (substin:substitution) (subst:substitution) 
                          (s:substrate) (k:infostrate). 
          ((Includes xs (Domain subst)) && 
-          (Includes xs (FreeVarsPoly (PolySubst i substin))) &&
           (InfonLogic.polyentails s k [] (PolySubst (PolySubst i substin) subst)))
       => HoldsOne substin xs (If i) subst
 
 assume Holds_upon: forall (xs:vars) (pat:infon) (substin:substitution) (subst:substitution) (c:communication). 
          ((Includes xs (Domain subst)) &&
-          (Includes xs (FreeVarsPoly (PolySubst pat substin))) &&
           ((PolySubst (PolySubst pat substin) subst)=c))
       => HoldsOne substin xs (Upon pat) subst
 
 type HoldsMany :: vars => list condition => substitution => E
-assume forall (xs:vars). HoldsMany xs [] EmptySubst
+assume forall (xs:vars). HoldsMany xs [] []
 assume forall (xs:vars) (c:condition) (cs:conditions) 
                (s0:substitution) (s1:substitution).
           (HoldsMany xs cs s0) && (HoldsOne s0 xs c s1)
          => HoldsMany xs (c::cs) s1
 type Holds :: _ = fun (xs:vars) (cs:list condition) (s:substitution) => 
     ((Includes xs (Domain s)) && (Includes (Domain s) xs) && (HoldsMany xs cs s))
-
 (* -------------------------------------------------------------------------------- *)
 (* Spec: Enabled actions *)
 (* -------------------------------------------------------------------------------- *)
@@ -73,18 +99,26 @@ assume forall (me:principal) (p:principal) (i:infon).
           (Enabled (Send (Const (PrincipalConstant p)) i) && Crypto.IsMe me) 
        => SaysTo me p i
 
+type ruleAction :: _ = (fun (xs:vars) (cs:conditions) => 
+                        (a:action{forall (subst:substitution). Holds xs cs subst => (Enabled (ActionSubst a subst))}))
+type ruleActions :: _ = (fun (xs:vars) (cs:conditions) => (list (ruleAction xs cs)))
+
 type rule =
   | Rule : xs:vars 
         -> cs:conditions 
-        -> acts:list (a:action{forall (subst:substitution). Holds xs cs subst => (Enabled (ActionSubst a subst))})
+        -> list (ruleAction xs cs)
         -> rule
-
-type rules = list rule
+type WFR :: rule => P = 
+  | WFR_Rule : xs:vars -> cs:conditions{Binds cs xs} -> acts:ruleActions xs cs
+            -> ForallL condition cs  (WFCond xs) 
+            -> ForallL (ruleAction xs cs) acts (WFAct xs)
+            -> WFR (Rule xs cs acts)
+type wfrule = r:rule{WFR r}
 
 (* ================= Wrapping external functions ===================== *)
 type substholdsone :: _ = (fun (xs:vars) (c:condition) (s0:substitution) => (s:substitution{HoldsOne s0 xs c s}))
 type substholdsmany :: _ = (fun (xs:vars) (cs:conditions) => (s:substitution{HoldsMany xs cs s}))
-type substholdsex  :: _ = (fun (xs:vars) (c:condition) (sl:substitutions) => (s:substitution{exists (s0:substitution). In s0 sl && HoldsOne s0 xs c s}))
+(* type substholdsex  :: _ = (fun (xs:vars) (c:condition) (sl:substitutions) => (s:substitution{exists (s0:substitution). In s0 sl && HoldsOne s0 xs c s})) *)
 
 val derive: u:vars
           -> goal:infon
@@ -94,8 +128,7 @@ let derive u goal subst0 =
   let s = State.getSubstrate () in
   let k = State.getInfostrate () in 
   let goal' = polysubst goal subst0 in 
-    if (includes u (domain subst0)) &&
-       (includes u (freeVarsPoly goal')) (* TODO: push into pre-condition *)
+    if (includes u (domain subst0)) (* TODO: push into pre-condition *)
     then match InfonLogic.deriveQuant u s k subst0 goal with
       | None -> []
       | Some ((subst, pf)) -> [subst]
@@ -149,23 +182,16 @@ val matchComm : comm:communication
              -> s0:substitution 
              -> list (substholdsone xs (Upon pat) s0)
 let matchComm (comm:communication) xs pat s0 = 
-  if includes xs (freeVarsPoly (polysubst pat s0))
-  then match Unify.match_pattern comm s0 xs pat with
+  match Unify.match_pattern comm s0 xs pat with
     | None -> []
     | Some s1 -> [s1]
-  else []
 
 let matchComms xs pat s = collect (fun comm -> matchComm comm xs pat s) (!comms)
   
-val evalCondOne: xs:vars -> s0:substitution -> c:condition -> list (substholdsone xs c s0)
-let evalCondOne xs s0 c = match c with 
+val evalCond: xs:vars -> s0:substitution -> c:condition -> list (substholdsone xs c s0)
+let evalCond xs s0 c = match c with 
   | If pat -> derive xs pat s0
   | Upon pat -> matchComms xs pat s0
-
-val evalCond: xs:vars -> sl:substitutions -> c:condition -> list (substholdsex xs c sl)
-let evalCond xs sl c = match c with 
-  | If pat -> collect_in sl (fun s0 -> map (fun (x:substholdsone xs c s0) -> (x:substholdsex xs c sl)) (derive xs pat s0))
-  | Upon pat -> collect_in sl (fun s0 -> map (fun (x:substholdsone xs c s0) -> (x:substholdsex xs c sl)) (matchComms xs pat s0))
 
 val evalConds: xs:vars -> cs:conditions -> list (substholdsmany xs cs)
 let rec evalConds xs cs =
@@ -175,7 +201,7 @@ let rec evalConds xs cs =
         let sl' = evalConds xs cstl in
           collect (fun (s0:substitution{HoldsMany xs cstl s0}) ->  (* abbrevs don't work here ... fix *)
                      map (fun (s1:substitution{HoldsOne s0 xs c s1}) -> (s1:substholdsmany xs (c::cstl)))
-                       (evalCondOne xs s0 c))
+                       (evalCond xs s0 c))
             sl' 
 
 val holds: xs:vars -> cs:conditions -> list (s:substitution{Holds xs cs s})
@@ -199,12 +225,18 @@ let substAction s a =
 let crev x f = collect f x
 let cmap x f = map f x 
 
-val enabledActions : r:rule -> list (a:action{Enabled a})
+val enabledActions : wfrule -> list (a:action{Enabled a})
 let enabledActions r = match r with 
-  | Rule xs cs acts -> crev acts (fun a -> 
-                                    cmap (holds xs cs)
-                                      (fun s -> let a':(a':action{Enabled a'}) = substAction s a in a'))
-
+  | Rule xs cs acts -> 
+      crev acts (fun (a:action{forall (subst:substitution). Holds xs cs subst => (Enabled (ActionSubst a subst))}) -> 
+                   cmap (holds xs cs)
+                     (fun (s:substitution{Holds xs cs s}) -> 
+                         let a':(a':action{Enabled a'}) = substAction s a in  a'))
+                           (* assert (Holds xs cs s); *)
+                           (* assert (a'=(ActionSubst a s)); *)
+                           (* assert (Enabled a'); *)
+                           (* a')) *)
+        
 let allEnabledActions rs = collect enabledActions rs
 
 val asPrincipal: p:term -> q:principal{p=(Const (PrincipalConstant q))}
@@ -220,16 +252,66 @@ let applyAction b a =
     | Fwd p i -> fwd (asPrincipal p) i
     | Send p i -> send (asPrincipal p) i
 
-val until_fix: rules -> unit
+val until_fix: list wfrule -> unit
 let rec until_fix rs = 
   let actions = allEnabledActions rs in
     if fold_left applyAction false actions
     then until_fix rs 
     else ()
   
-val run: rules -> unit
-let rec run rs = 
+val go: list wfrule -> unit
+let rec go rs = 
   let _ = clear_out_buffer () in 
   let _ = get_communications () in (* blocks until new comms arrive *)
   let _ = until_fix rs in
-    run rs
+    go rs
+
+let varsOne c : v:vars{v=(VarsCond c)} = match c with 
+  | If (MonoTerm i) -> freeVars i
+  | If (ForallT xs i) -> freeVars i
+  | Upon (MonoTerm i) -> freeVars i
+  | Upon (ForallT xs i) -> freeVars i 
+
+val vars: c:conditions -> v:vars{v=(VarsConds c)}
+let rec vars = function 
+  | [] -> []
+  | c::rest ->  append (varsOne c) (vars rest)
+        
+val checkWFR: r:rule -> b:bool{b=true => WFR r}
+let checkWFR = function 
+  | Rule xs cs acts -> 
+      let wfCond ys c : option (WFCond ys c) = match c with 
+        | If i -> (match Typing.doPolyTyping ys i with 
+                     | MkPartial pf -> Some (WFCond_If ys i pf))
+        | Upon i -> (match Typing.doPolyTyping ys i with 
+                       | MkPartial pf -> Some (WFCond_Upon ys i pf)) in
+      let wfAct ys a : option (WFAct ys a) = match a with 
+        | Learn i -> (match Typing.doPolyTyping ys i with 
+                        | MkPartial pf -> Some (WFAct_Learn ys i pf))
+        | Drop i -> (match Typing.doPolyTyping ys i with 
+                       | MkPartial pf -> Some (WFAct_Drop ys i pf))
+        | Fwd p i -> 
+            let (tp, pfp) = Typing.doTyping ys p in 
+              if tp=Principal
+              then match Typing.doPolyTyping ys i with
+                | MkPartial pf -> Some (WFAct_Fwd ys p i pfp pf)
+              else None            
+        | Send p i -> 
+            let (tp, pfp) = Typing.doTyping ys p in 
+              if tp=Principal
+              then match Typing.doPolyTyping ys i with
+                | MkPartial pf -> Some (WFAct_Send ys p i pfp pf)
+              else None in
+      let wfconds = mapL_p<condition, (WFCond xs)> (wfCond xs) cs in 
+      let wfacts = mapL_p<(ruleAction xs cs), (WFAct xs)> (wfAct xs) acts in 
+        match wfconds, wfacts with 
+          | Some pf1, Some pf2 when includes (vars cs) xs -> 
+              let pf = WFR_Rule xs cs acts pf1 pf2 in true
+          | _ -> false
+
+val tcrule: rule -> wfrule
+let tcrule r = if checkWFR r then r else raise "Ill-typed rule"
+
+val run : list rule -> unit
+let run rules = go (map tcrule rules)
+
